src/computational_monads/simulation_semantics/constructions/logging.lean
@@ -1,0 +1,91 @@
+import computational_monads.constructions.uniform_select
+import computational_monads.simulation_semantics.simulate
+import computational_monads.simulation_semantics.stateless_oracle
+import computational_monads.simulation_semantics.constructions.query_log
+
+open oracle_comp oracle_spec
+
+variables {spec spec' spec'' : oracle_spec} {A B C : Type}
+
+section logging_oracle
+
+/-- Extend the state of a simulation oracle to also track the inputs and outputs of queries.
+  The actual oracle calls are forwarded directly to the original oracle. -/
+def logging_simulation_oracle (spec : oracle_spec) [spec.computable] : 
+  simulation_oracle spec spec :=
+{ S := query_log spec,
+  o := λ i ⟨t, log⟩, do { u ← query i t, return (u, log.log_query i t u) } }
+
+namespace logging_simulation_oracle
+
+@[simp]
+lemma simulate_pure [spec.computable] (a : A) (log : query_log spec) :
+  simulate (logging_simulation_oracle _) (return a) log = return ⟨a, log⟩ :=
+rfl
+
+@[simp]
+lemma simulate_query [spec.computable] (i : spec.ι) (t : spec.domain i) (log : query_log spec) :
+  simulate (logging_simulation_oracle _) (query i t) log =
+    do { u ← query i t, return (u, log.log_query i t u) } :=
+rfl
+
+@[simp]
+lemma simulate_bind [spec.computable] (oa : oracle_comp spec A) (ob : A → oracle_comp spec B) (log : query_log spec) :
+  simulate (logging_simulation_oracle _) (oa >>= ob) log =
+    (simulate (logging_simulation_oracle _) oa log) >>=
+      (λ x, simulate (logging_simulation_oracle _) (ob x.1) x.2) :=
+rfl
+
+@[simp]
+lemma eval_distribution_fst_simulate [spec.computable] [spec.finite_range] (oa : oracle_comp spec A) (log : query_log spec) :
+  ⟦ (simulate (logging_simulation_oracle _) oa log) >>= (λ a, return a.1) ⟧ = ⟦ oa ⟧ :=
+begin
+  induction oa,
+  {
+    simp,
+    refine (pmf.pure_bind _ _).trans _,
+    simp,
+  },
+  {
+    sorry,
+  },
+  {
+    sorry
+  }
+end
+
+end logging_simulation_oracle
+
+end logging_oracle
+
+section seeded_oracle
+
+/-- Use the first element of the `seed` as the query result if inputs match.
+  If the query values don't match then throw away the seed as computation has diverged.
+  Using this with a log from a previous computation ensures they behave identically. -/
+def seeded_simulation_oracle (spec : oracle_spec) [computable spec] :
+  simulation_oracle spec spec :=
+{ S := query_log spec,
+  o := λ i ⟨t, seed⟩, match seed.lookup_fst i t with
+    | none := functor.map (λ u, (u, query_log.init spec)) (query i t)
+    | (some u) := return (u, seed.remove_head i)
+    end }
+
+namespace seeded_simulation_oracle
+
+end seeded_simulation_oracle
+
+end seeded_oracle
+
+section caching_oracle
+
+-- TODO: make this a extension property instead.
+def caching_simulation_oracle (spec : oracle_spec) [spec.computable] :
+  simulation_oracle spec spec :=
+{ S := query_log spec,
+  o := λ i ⟨t, log⟩, match log.lookup i t with
+  | (some u) := return (u, log) -- Return the cached value if it already exists
+  | none := do { u ← query i t, return (u, log.log_query i t u) }
+  end }
+
+end caching_oracle
